common/ProgramLSim.v
@@ -17,7 +17,7 @@ Proof.
 Qed.
 
 (* lifting function simulation to program simulation *)
-Section PROGRAM_SIM.
+Section PROGRAM_LSIM.
 
 Variable (fundefT_src F_src V_src:Type).
 Variable (fundef_src_dec: fundef_decT fundefT_src F_src).
@@ -40,9 +40,9 @@ Let fundef_sig_tgt (fundef:fundefT_tgt): signature :=
   end.
 
 Variable (transf_V: forall (v:V_src), res V_tgt).
-Let V_sim (v_src:V_src) (v_tgt:V_tgt) := transf_V v_src = OK v_tgt.
+Let V_lsim (v_src:V_src) (v_tgt:V_tgt) := transf_V v_src = OK v_tgt.
 
-Definition F_simT :=
+Definition F_lsimT :=
   forall
     (fprog_src:program fundefT_src V_src)
     (fprog_tgt:program fundefT_tgt V_tgt)
@@ -50,144 +50,144 @@ Definition F_simT :=
 
 Section CORE.
 
-Variable (F_sim:F_simT).
+Variable (F_lsim:F_lsimT).
 Variable (prog_src:program fundefT_src V_src).
 Variable (prog_tgt:program fundefT_tgt V_tgt).
 
-Inductive globvar_sim (v_src:globvar V_src) (v_tgt:globvar V_tgt): Prop :=
-| globvar_sim_intro
+Inductive globvar_lsim (v_src:globvar V_src) (v_tgt:globvar V_tgt): Prop :=
+| globvar_lsim_intro
     (Hv: transf_globvar transf_V v_src = OK v_tgt)
 .
 
 (** simulation *)
-Inductive globfun_sim
+Inductive globfun_lsim
           (g_src:fundefT_src) (g_tgt:fundefT_tgt): Prop :=
-| globfun_sim_i
+| globfun_lsim_i
     f_src f_tgt
     (Hsrc: fundef_src_dec g_src = inl f_src)
     (Htgt: fundef_tgt_dec g_tgt = inl f_tgt)
     (Hsim: forall fprog_src fprog_tgt
                   (Hfprog_src: program_linkeq fundef_src_dec prog_src fprog_src)
                   (Hfprog_tgt: program_linkeq fundef_tgt_dec prog_tgt fprog_tgt),
-             F_sim fprog_src fprog_tgt f_src f_tgt /\
+             F_lsim fprog_src fprog_tgt f_src f_tgt /\
              F_sig_src f_src = F_sig_tgt f_tgt)
-| globfun_sim_e
+| globfun_lsim_e
     ef
     (Hsrc: fundef_src_dec g_src = inr ef)
     (Htgt: fundef_tgt_dec g_tgt = inr ef)
 .
 
-Inductive globdef_sim:
+Inductive globdef_lsim:
   forall (g_src:globdef fundefT_src V_src) (g_tgt:globdef fundefT_tgt V_tgt), Prop :=
-| globdef_sim_fun
-    f_src f_tgt (Hf: globfun_sim f_src f_tgt):
-    globdef_sim (Gfun f_src) (Gfun f_tgt)
-| globdef_sim_var
-    v_src v_tgt (Hv: globvar_sim v_src v_tgt):
-    globdef_sim (Gvar v_src) (Gvar v_tgt)
+| globdef_lsim_fun
+    f_src f_tgt (Hf: globfun_lsim f_src f_tgt):
+    globdef_lsim (Gfun f_src) (Gfun f_tgt)
+| globdef_lsim_var
+    v_src v_tgt (Hv: globvar_lsim v_src v_tgt):
+    globdef_lsim (Gvar v_src) (Gvar v_tgt)
 .
 
-Definition globdefs_sim
+Definition globdefs_lsim
            (defs_src:PTree.t (globdef fundefT_src V_src))
            (defs_tgt:PTree.t (globdef fundefT_tgt V_tgt)): Prop :=
   forall i,
     match PTree.get i defs_src, PTree.get i defs_tgt with
-      | Some g1, Some g2 => globdef_sim g1 g2
+      | Some g1, Some g2 => globdef_lsim g1 g2
       | None, None => True
       | _, _ => False
     end.
 
-Definition globdef_list_sim
+Definition globdef_list_lsim
            (defs_src:list (positive * globdef fundefT_src V_src))
            (defs_tgt:list (positive * globdef fundefT_tgt V_tgt)): Prop :=
   list_forall2
     (fun g_src g_tgt =>
        fst g_src = fst g_tgt /\
-       globdef_sim (snd g_src) (snd g_tgt))
+       globdef_lsim (snd g_src) (snd g_tgt))
     defs_src defs_tgt.
 
-Definition program_sim_aux: Prop :=
-  globdef_list_sim prog_src.(prog_defs) prog_tgt.(prog_defs) /\
+Definition program_lsim_aux: Prop :=
+  globdef_list_lsim prog_src.(prog_defs) prog_tgt.(prog_defs) /\
   prog_src.(prog_main) = prog_tgt.(prog_main).
 
 End CORE.
 
 (** an instantiation of weak simulation: matching any function definitions *)
-Definition program_weak_sim := program_sim_aux (fun _ _ _ _ => True).
+Definition program_weak_lsim := program_lsim_aux (fun _ _ _ _ => True).
 
-(** properties on F_sim and simulation *)
-Lemma globfun_sim_le
-      (F_sim1 F_sim2:F_simT)
+(** properties on F_lsim and simulation *)
+Lemma globfun_lsim_le
+      (F_lsim1 F_lsim2:F_lsimT)
       (prog1_src prog2_src:program fundefT_src V_src)
       (prog1_tgt prog2_tgt:program fundefT_tgt V_tgt)
-      (HF_sim: F_sim1 <4= F_sim2)
+      (HF_lsim: F_lsim1 <4= F_lsim2)
       (Hprog_src: program_linkeq fundef_src_dec prog1_src prog2_src)
       (Hprog_tgt: program_linkeq fundef_tgt_dec prog1_tgt prog2_tgt):
-  (globfun_sim F_sim1 prog1_src prog1_tgt) <2= (globfun_sim F_sim2 prog2_src prog2_tgt).
+  (globfun_lsim F_lsim1 prog1_src prog1_tgt) <2= (globfun_lsim F_lsim2 prog2_src prog2_tgt).
 Proof.
   intros. inv PR.
-  - eapply globfun_sim_i; eauto.
+  - eapply globfun_lsim_i; eauto.
     intros. exploit Hsim; eauto. intros [Hsim1 Hsig].
-    split; auto. apply HF_sim. eapply Hsim.
+    split; auto. apply HF_lsim. eapply Hsim.
     + rewrite Hprog_src. auto.
     + rewrite Hprog_tgt. auto.
-  - eapply globfun_sim_e; eauto.
+  - eapply globfun_lsim_e; eauto.
 Qed.
 
-Lemma globdef_sim_le
-      (F_sim1 F_sim2:F_simT)
+Lemma globdef_lsim_le
+      (F_lsim1 F_lsim2:F_lsimT)
       (prog1_src prog2_src:program fundefT_src V_src)
       (prog1_tgt prog2_tgt:program fundefT_tgt V_tgt)
-      (HF_sim: F_sim1 <4= F_sim2)
+      (HF_lsim: F_lsim1 <4= F_lsim2)
       (Hprog_src: program_linkeq fundef_src_dec prog1_src prog2_src)
       (Hprog_tgt: program_linkeq fundef_tgt_dec prog1_tgt prog2_tgt):
-  (globdef_sim F_sim1 prog1_src prog1_tgt) <2= (globdef_sim F_sim2 prog2_src prog2_tgt).
+  (globdef_lsim F_lsim1 prog1_src prog1_tgt) <2= (globdef_lsim F_lsim2 prog2_src prog2_tgt).
 Proof.
   intros. inv PR.
-  - eapply globdef_sim_fun; eauto.
-    eapply globfun_sim_le; eauto.
-  - eapply globdef_sim_var; eauto.
+  - eapply globdef_lsim_fun; eauto.
+    eapply globfun_lsim_le; eauto.
+  - eapply globdef_lsim_var; eauto.
 Qed.
 
-Lemma globdef_list_sim_le
-      (F_sim1 F_sim2:F_simT)
+Lemma globdef_list_lsim_le
+      (F_lsim1 F_lsim2:F_lsimT)
       (prog1_src prog2_src:program fundefT_src V_src)
       (prog1_tgt prog2_tgt:program fundefT_tgt V_tgt)
-      (HF_sim: F_sim1 <4= F_sim2)
+      (HF_lsim: F_lsim1 <4= F_lsim2)
       (Hprog_src: program_linkeq fundef_src_dec prog1_src prog2_src)
       (Hprog_tgt: program_linkeq fundef_tgt_dec prog1_tgt prog2_tgt):
-  (globdef_list_sim F_sim1 prog1_src prog1_tgt) <2= (globdef_list_sim F_sim2 prog2_src prog2_tgt).
+  (globdef_list_lsim F_lsim1 prog1_src prog1_tgt) <2= (globdef_list_lsim F_lsim2 prog2_src prog2_tgt).
 Proof.
   intros.
   eapply list_forall2_imply; eauto. simpl. intros.
   destruct H1, v1, v2. simpl in *. subst.
-  split; auto. eapply globdef_sim_le; eauto.
+  split; auto. eapply globdef_lsim_le; eauto.
 Qed.
 
-Lemma program_sim_aux_le
-      (F_sim1 F_sim2:F_simT)
-      (HF_sim: F_sim1 <4= F_sim2):
-  (program_sim_aux F_sim1) <2= (program_sim_aux F_sim2).
+Lemma program_lsim_aux_le
+      (F_lsim1 F_lsim2:F_lsimT)
+      (HF_lsim: F_lsim1 <4= F_lsim2):
+  (program_lsim_aux F_lsim1) <2= (program_lsim_aux F_lsim2).
 Proof.
   intros prog_src prog_tgt Hsim.
   destruct prog_src as [defs_src main_src].
   destruct prog_tgt as [defs_tgt main_tgt].
   destruct Hsim as [Hdefs Hmain].
   simpl in *. subst. split; auto.
-  eapply globdef_list_sim_le; simpl; eauto.
+  eapply globdef_list_lsim_le; simpl; eauto.
   reflexivity. reflexivity.
 Qed.
 
-(** globdefs_sim and globdef_list_sim *)
+(** globdefs_lsim and globdef_list_lsim *)
 
-Lemma globdefs_sim_globdef_list_sim
-      (F_sim:F_simT)
+Lemma globdefs_lsim_globdef_list_lsim
+      (F_lsim:F_lsimT)
       (fprog_src:program fundefT_src V_src)
       (fprog_tgt:program fundefT_tgt V_tgt)
       (defs_src: PTree.t (globdef fundefT_src V_src))
       (defs_tgt: PTree.t (globdef fundefT_tgt V_tgt))
-      (Hsim: globdefs_sim F_sim fprog_src fprog_tgt defs_src defs_tgt):
-  globdef_list_sim F_sim fprog_src fprog_tgt (PTree.elements defs_src) (PTree.elements defs_tgt).
+      (Hsim: globdefs_lsim F_lsim fprog_src fprog_tgt defs_src defs_tgt):
+  globdef_list_lsim F_lsim fprog_src fprog_tgt (PTree.elements defs_src) (PTree.elements defs_tgt).
 Proof.
   apply PTree.elements_canonical_order; intros.
   - exploit Hsim. instantiate (1 := i). rewrite H. intro X.
@@ -198,16 +198,16 @@ Proof.
     eexists. split; eauto.
 Qed.
 
-Lemma globdef_list_sim_globdefs_sim
-      (F_sim:F_simT)
+Lemma globdef_list_lsim_globdefs_lsim
+      (F_lsim:F_lsimT)
       (fprog_src:program fundefT_src V_src)
       (fprog_tgt:program fundefT_tgt V_tgt)
       (defs_src: list (positive * (globdef fundefT_src V_src)))
       (defs_tgt: list (positive * (globdef fundefT_tgt V_tgt)))
-      (Hsim: globdef_list_sim F_sim fprog_src fprog_tgt defs_src defs_tgt):
-  globdefs_sim F_sim fprog_src fprog_tgt (PTree.unelements defs_src) (PTree.unelements defs_tgt).
+      (Hsim: globdef_list_lsim F_lsim fprog_src fprog_tgt defs_src defs_tgt):
+  globdefs_lsim F_lsim fprog_src fprog_tgt (PTree.unelements defs_src) (PTree.unelements defs_tgt).
 Proof.
-  unfold globdefs_sim, globdef_list_sim in *. intro i.
+  unfold globdefs_lsim, globdef_list_lsim in *. intro i.
   rewrite ? PTree.guespec. apply list_forall2_rev in Hsim.
   revert Hsim i. generalize (rev defs_src) (rev defs_tgt).
   induction l; intros l0 Hsim i; inv Hsim; simpl; auto.
@@ -228,28 +228,28 @@ Ltac simplify_decs :=
         rewrite Hl in Hr; inv Hr
     end.
 
-Lemma link_globdefs_sim
-      (F_sim:F_simT)
+Lemma link_globdefs_lsim
+      (F_lsim:F_lsimT)
       (main:positive)
       (defs1_src defs2_src:list (positive * globdef fundefT_src V_src))
       (defs1_tgt defs2_tgt:list (positive * globdef fundefT_tgt V_tgt))
       defs_src (Hdefs_src: link_globdefs fundef_src_dec V_src_dec (PTree.unelements defs1_src) (PTree.unelements defs2_src) = Some defs_src)
-      (H1: globdefs_sim
-             F_sim
+      (H1: globdefs_lsim
+             F_lsim
              (mkprogram defs1_src main)
              (mkprogram defs1_tgt main)
              (PTree.unelements defs1_src)
              (PTree.unelements defs1_tgt))
-      (H2: globdefs_sim
-             F_sim
+      (H2: globdefs_lsim
+             F_lsim
              (mkprogram defs2_src main)
              (mkprogram defs2_tgt main)
              (PTree.unelements defs2_src)
              (PTree.unelements defs2_tgt)):
   exists defs_tgt,
     link_globdefs fundef_tgt_dec V_tgt_dec (PTree.unelements defs1_tgt) (PTree.unelements defs2_tgt) = Some defs_tgt /\
-    globdefs_sim
-      F_sim
+    globdefs_lsim
+      F_lsim
       (mkprogram (PTree.elements defs_src) main)
       (mkprogram (PTree.elements defs_tgt) main)
       defs_src defs_tgt.
@@ -274,13 +274,13 @@ Proof.
     { destruct Hdefs_src as [[]|[]], Hdefs_tgt as [[]|[]]; subst;
       repeat
         match goal with
-          | [H: globfun_sim _ _ _ _ _ |- _] => inv H
+          | [H: globfun_lsim _ _ _ _ _ |- _] => inv H
           | [H1: fundef_src_dec ?f = _, H2: fundef_src_dec ?f = _ |- _] =>
             rewrite H1 in H2; inv H2
           | [H1: fundef_tgt_dec ?f = _, H2: fundef_tgt_dec ?f = _ |- _] =>
             rewrite H1 in H2; inv H2
         end.
-      - eapply globdef_sim_le; eauto.
+      - eapply globdef_lsim_le; eauto.
         + split; auto. unfold globdef_list_linkeq. rewrite Hle2_src.
           repeat intro. exists def1. split; [|reflexivity].
           simpl. rewrite PTree.unelements_elements. auto.
@@ -290,13 +290,13 @@ Proof.
       - inv H; inv H1; inv H2; inv H3; inv Hv; inv Hv0; repeat constructor;
         repeat
           match goal with
-            | [H: globfun_sim _ _ _ _ _ |- _] => inv H
+            | [H: globfun_lsim _ _ _ _ _ |- _] => inv H
             | [H1: fundef_src_dec ?f = _, H2: fundef_src_dec ?f = _ |- _] =>
               rewrite H1 in H2; inv H2
             | [H1: fundef_tgt_dec ?f = _, H2: fundef_tgt_dec ?f = _ |- _] =>
               rewrite H1 in H2; inv H2
           end.
-        + eapply globfun_sim_e; eauto.
+        + eapply globfun_lsim_e; eauto.
         + inv Hv1. destruct v1, v2; simpl in *; subst.
           unfold transf_globvar in *. simpl in *.
           destruct (transf_V gvar_info0); simpl in *; inv Hv; inv Hv0.
@@ -304,13 +304,13 @@ Proof.
       - inv H; inv H1; inv H2; inv H3; inv Hv; inv Hv0; repeat constructor;
         repeat
           match goal with
-            | [H: globfun_sim _ _ _ _ _ |- _] => inv H
+            | [H: globfun_lsim _ _ _ _ _ |- _] => inv H
             | [H1: fundef_src_dec ?f = _, H2: fundef_src_dec ?f = _ |- _] =>
               rewrite H1 in H2; inv H2
             | [H1: fundef_tgt_dec ?f = _, H2: fundef_tgt_dec ?f = _ |- _] =>
               rewrite H1 in H2; inv H2
           end.
-        + eapply globfun_sim_e; eauto.
+        + eapply globfun_lsim_e; eauto.
         + inv Hv1. destruct v1, v2; simpl in *; subst.
           unfold transf_globvar in *. simpl in *.
           destruct (transf_V gvar_info0); simpl in *; inv Hv; inv Hv0.
@@ -318,13 +318,13 @@ Proof.
       - inv H; inv H1; inv H2; inv H3; inv Hv; inv Hv0; repeat constructor;
         repeat
           match goal with
-            | [H: globfun_sim _ _ _ _ _ |- _] => inv H
+            | [H: globfun_lsim _ _ _ _ _ |- _] => inv H
             | [H1: fundef_src_dec ?f = _, H2: fundef_src_dec ?f = _ |- _] =>
               rewrite H1 in H2; inv H2
             | [H1: fundef_tgt_dec ?f = _, H2: fundef_tgt_dec ?f = _ |- _] =>
               rewrite H1 in H2; inv H2
           end.
-        + eapply globfun_sim_i; eauto. intros. apply Hsim.
+        + eapply globfun_lsim_i; eauto. intros. apply Hsim.
           * destruct Hfprog_src as [Hfdefs_src ?]. simpl in *. subst.
             split; auto. unfold globdef_list_linkeq in *.
             rewrite Hle1_src, <- Hfdefs_src.
@@ -335,13 +335,13 @@ Proof.
             rewrite Hle1_tgt, <- Hfdefs_tgt.
             repeat intro. exists def1. split; [|reflexivity].
             rewrite PTree.unelements_elements. auto.
-        + eapply globfun_sim_e; eauto.
+        + eapply globfun_lsim_e; eauto.
         + inv Hv1. destruct v1, v2; simpl in *; subst.
           unfold transf_globvar in *. simpl in *.
           destruct (transf_V gvar_info0); simpl in *; inv Hv; inv Hv0.
           inv Hv2. simpl in *. subst. auto.
     }
-    { eapply globdef_sim_le; eauto.
+    { eapply globdef_lsim_le; eauto.
       - split; auto. unfold globdef_list_linkeq. rewrite Hle1_src.
         repeat intro. exists def1. split; [|reflexivity].
         simpl. rewrite PTree.unelements_elements. auto.
@@ -349,7 +349,7 @@ Proof.
         repeat intro. exists def1. split; [|reflexivity].
         simpl. rewrite PTree.unelements_elements. auto.
     }
-    { eapply globdef_sim_le; eauto.
+    { eapply globdef_lsim_le; eauto.
       - split; auto. unfold globdef_list_linkeq. rewrite Hle2_src.
         repeat intro. exists def1. split; [|reflexivity].
         simpl. rewrite PTree.unelements_elements. auto.
@@ -392,66 +392,66 @@ Proof.
   }
 Qed.
 
-Lemma link_globdef_list_sim
-      (F_sim:F_simT)
+Lemma link_globdef_list_lsim
+      (F_lsim:F_lsimT)
       (main:positive)
       (defs1_src defs2_src:list (positive * globdef fundefT_src V_src))
       (defs1_tgt defs2_tgt:list (positive * globdef fundefT_tgt V_tgt))
       defs_src (Hdefs_src: link_globdef_list fundef_src_dec V_src_dec defs1_src defs2_src = Some defs_src)
-      (H1: globdef_list_sim
-             F_sim
+      (H1: globdef_list_lsim
+             F_lsim
              (mkprogram defs1_src main)
              (mkprogram defs1_tgt main)
              defs1_src defs1_tgt)
-      (H2: globdef_list_sim
-             F_sim
+      (H2: globdef_list_lsim
+             F_lsim
              (mkprogram defs2_src main)
              (mkprogram defs2_tgt main)
              defs2_src defs2_tgt):
   exists defs_tgt,
     link_globdef_list fundef_tgt_dec V_tgt_dec defs1_tgt defs2_tgt = Some defs_tgt /\
-    globdef_list_sim
-      F_sim
+    globdef_list_lsim
+      F_lsim
       (mkprogram defs_src main)
       (mkprogram defs_tgt main)
       defs_src defs_tgt.
 Proof.
-  apply globdef_list_sim_globdefs_sim in H1.
-  apply globdef_list_sim_globdefs_sim in H2.
+  apply globdef_list_lsim_globdefs_lsim in H1.
+  apply globdef_list_lsim_globdefs_lsim in H2.
   unfold link_globdef_list in Hdefs_src.
   match goal with
     | [H: context[link_globdefs ?fundef_dec ?V_dec ?defs1 ?defs2] |- _] =>
       destruct (link_globdefs fundef_dec V_dec defs1 defs2) as [defs|] eqn:Hdefs; inv H
   end.
-  exploit link_globdefs_sim; eauto. intros [defs_tgt [Hdefs_tgt Hsim]].
+  exploit link_globdefs_lsim; eauto. intros [defs_tgt [Hdefs_tgt Hsim]].
   unfold link_globdef_list. rewrite Hdefs_tgt. eexists. split; eauto.
-  apply globdefs_sim_globdef_list_sim. auto.
+  apply globdefs_lsim_globdef_list_lsim. auto.
 Qed.
 
 Section DEF.
 
-Variable (F_sim:F_simT).
+Variable (F_lsim:F_lsimT).
 
-Definition F_future_sim :=
+Definition F_future_lsim :=
   fun fprog_src fprog_tgt f_src f_tgt =>
-    forall (Hfprog: program_weak_sim fprog_src fprog_tgt),
-    F_sim fprog_src fprog_tgt f_src f_tgt.
+    forall (Hfprog: program_weak_lsim fprog_src fprog_tgt),
+    F_lsim fprog_src fprog_tgt f_src f_tgt.
 
-Definition program_sim
+Definition program_lsim
            (prog_src: program fundefT_src V_src)
            (prog_tgt: program fundefT_tgt V_tgt): Prop :=
-  globdef_list_sim F_future_sim prog_src prog_tgt prog_src.(prog_defs) prog_tgt.(prog_defs) /\
+  globdef_list_lsim F_future_lsim prog_src prog_tgt prog_src.(prog_defs) prog_tgt.(prog_defs) /\
   prog_src.(prog_main) = prog_tgt.(prog_main).
 
-Lemma link_program_sim
+Lemma link_program_lsim
       (p1_src p2_src:program fundefT_src V_src)
       (p1_tgt p2_tgt:program fundefT_tgt V_tgt)
       p_src (Hp_src: link_program fundef_src_dec V_src_dec p1_src p2_src = Some p_src)
-      (H1: program_sim p1_src p1_tgt)
-      (H2: program_sim p2_src p2_tgt):
+      (H1: program_lsim p1_src p1_tgt)
+      (H2: program_lsim p2_src p2_tgt):
   exists p_tgt,
     link_program fundef_tgt_dec V_tgt_dec p1_tgt p2_tgt = Some p_tgt /\
-    program_sim p_src p_tgt.
+    program_lsim p_src p_tgt.
 Proof.
   destruct p1_src as [defs1_src main1_src].
   destruct p1_tgt as [defs1_tgt main1_tgt].
@@ -462,38 +462,38 @@ Proof.
   destruct ((main1_tgt =? main2_tgt)%positive) eqn:Hmain; [|inv Hp_src].
   apply Pos.eqb_eq in Hmain. subst.
   destruct (link_globdef_list fundef_src_dec V_src_dec defs1_src defs2_src) as [def_list_src|] eqn:Hdef_list_src; inv Hp_src.
-  exploit link_globdef_list_sim; eauto. intros [defs_tgt [Hdefs_tgt Hsim]].
+  exploit link_globdef_list_lsim; eauto. intros [defs_tgt [Hdefs_tgt Hsim]].
   exists (mkprogram defs_tgt main2_tgt). rewrite Hdefs_tgt. split; auto.
   constructor; auto.
 Qed.
 
 End DEF.
 
-Lemma program_sim_le
-      (F_sim1 F_sim2:F_simT) (HF_sim: F_sim1 <4= F_sim2):
-  (program_sim F_sim1) <2= (program_sim F_sim2).
+Lemma program_lsim_le
+      (F_lsim1 F_lsim2:F_lsimT) (HF_lsim: F_lsim1 <4= F_lsim2):
+  (program_lsim F_lsim1) <2= (program_lsim F_lsim2).
 Proof.
   intros. destruct PR as [Hdefs Hmain]. split; auto.
-  eapply globdef_list_sim_le; eauto.
+  eapply globdef_list_lsim_le; eauto.
   - reflexivity.
   - reflexivity.
   - eapply list_forall2_imply; eauto. intros. simpl in *.
     destruct v1, v2, H1. simpl in *. subst.
     split; auto.
-    eapply globdef_sim_le; try reflexivity; [|eauto].
+    eapply globdef_lsim_le; try reflexivity; [|eauto].
     intros. repeat intro. specialize (PR Hfprog). auto.
 Qed.
 
-Inductive fundef_sig_sim (f_src:fundefT_src) (f_tgt:fundefT_tgt): Prop :=
-| fundef_sig_sim_intro
+Inductive fundef_sig_lsim (f_src:fundefT_src) (f_tgt:fundefT_tgt): Prop :=
+| fundef_sig_lsim_intro
     (Hsig: fundef_sig_src f_src = fundef_sig_tgt f_tgt)
 .
 
-Inductive fundef_weak_sim
+Inductive fundef_weak_lsim
           (ge_src:Genv.t fundefT_src V_src) (ge_tgt:Genv.t fundefT_tgt V_tgt)
           (f_src:fundefT_src) (f_tgt:fundefT_tgt): Prop :=
-| fundef_weak_sim_intro
-    (Hsig: fundef_sig_sim f_src f_tgt)
+| fundef_weak_lsim_intro
+    (Hsig: fundef_sig_lsim f_src f_tgt)
     b
     (Hsrc: Maps.PTree.get b ge_src.(Genv.genv_funs) = Some f_src)
     (Htgt: Maps.PTree.get b ge_tgt.(Genv.genv_funs) = Some f_tgt)
@@ -503,20 +503,20 @@ Section INITIALIZE.
 
 Variable (fprog_src: program fundefT_src V_src).
 Variable (fprog_tgt: program fundefT_tgt V_tgt).
-Variable (F_sim:F_simT).
-Variable (Hfprog: program_sim_aux F_sim fprog_src fprog_tgt).
+Variable (F_lsim:F_lsimT).
+Variable (Hfprog: program_lsim_aux F_lsim fprog_src fprog_tgt).
 
 Inductive match_fundef (f_src:fundefT_src) (f_tgt:fundefT_tgt): Prop :=
 | match_fundef_intro
-    (Hsig: fundef_sig_sim f_src f_tgt)
-    (Hsim: globfun_sim F_sim fprog_src fprog_tgt f_src f_tgt)
+    (Hsig: fundef_sig_lsim f_src f_tgt)
+    (Hsim: globfun_lsim F_lsim fprog_src fprog_tgt f_src f_tgt)
 .
 
 Let ge_src := Genv.globalenv fprog_src.
 Let ge_tgt := Genv.globalenv fprog_tgt.
 
-Lemma program_sim_match_program:
-  match_program match_fundef V_sim nil fprog_src.(prog_main) fprog_src fprog_tgt.
+Lemma program_lsim_match_program:
+  match_program match_fundef V_lsim nil fprog_src.(prog_main) fprog_src fprog_tgt.
 Proof.
   unfold match_program. destruct Hfprog as [Hfdefs Hmain].
   split; eauto. exists fprog_tgt.(prog_defs). split; [|rewrite app_nil_r; auto].
@@ -531,14 +531,14 @@ Proof.
   - destruct v_src, v_tgt. inv Hv. unfold transf_globvar in Hv0. simpl in *.
     destruct (transf_V gvar_info) eqn:Hgvar_info; inv Hv0. constructor; auto.
 Qed.
-Local Hint Resolve program_sim_match_program.
+Local Hint Resolve program_lsim_match_program.
 
 Lemma globalenvs_match:
-  Genv.match_genvs match_fundef V_sim nil (Genv.globalenv fprog_src) (Genv.globalenv fprog_tgt).
+  Genv.match_genvs match_fundef V_lsim nil (Genv.globalenv fprog_src) (Genv.globalenv fprog_tgt).
 Proof. eapply Genv.globalenvs_match; eauto. Qed.
 Local Hint Resolve globalenvs_match.
 
-Lemma program_sim_init_mem_match:
+Lemma program_lsim_init_mem_match:
   forall m,
     Genv.init_mem fprog_src = Some m ->
     Genv.init_mem fprog_tgt = Some m.
@@ -576,7 +576,7 @@ Lemma funct_ptr_translated:
   forall (b : block) (f : fundefT_src),
   Genv.find_funct_ptr (Genv.globalenv fprog_src) b = Some f ->
   exists tf : fundefT_tgt,
-  Genv.find_funct_ptr (Genv.globalenv fprog_tgt) b = Some tf /\ fundef_weak_sim ge_src ge_tgt f tf.
+  Genv.find_funct_ptr (Genv.globalenv fprog_tgt) b = Some tf /\ fundef_weak_lsim ge_src ge_tgt f tf.
 Proof.
   intros. exploit Genv.find_funct_ptr_match; eauto. intros [tf [Htf Hsim]].
   eexists. split; eauto. inv Hsim. inv Hsig. unfold Genv.find_funct_ptr in *.
@@ -587,7 +587,7 @@ Lemma funct_ptr_translated':
   forall (b : block) (f : fundefT_src),
   Genv.find_funct_ptr (Genv.globalenv fprog_src) b = Some f ->
   exists tf : fundefT_tgt,
-  Genv.find_funct_ptr (Genv.globalenv fprog_tgt) b = Some tf /\ globfun_sim F_sim fprog_src fprog_tgt f tf.
+  Genv.find_funct_ptr (Genv.globalenv fprog_tgt) b = Some tf /\ globfun_lsim F_lsim fprog_src fprog_tgt f tf.
 Proof.
   intros. exploit Genv.find_funct_ptr_match; eauto. intros [tf [Htf Hsim]].
   exists tf. split; auto. inv Hsim. auto.
@@ -596,7 +596,7 @@ Qed.
 Lemma functions_translated:
   forall v f,
   Genv.find_funct (Genv.globalenv fprog_src) v = Some f ->
-  exists tf, Genv.find_funct (Genv.globalenv fprog_tgt) v = Some tf /\ fundef_weak_sim ge_src ge_tgt f tf.
+  exists tf, Genv.find_funct (Genv.globalenv fprog_tgt) v = Some tf /\ fundef_weak_lsim ge_src ge_tgt f tf.
 Proof.
   intros. destruct v; inv H. 
   destruct (Int.eq_dec i Int.zero); inv H1.
@@ -604,7 +604,7 @@ Proof.
 Qed.
 
 Lemma sig_preserved:
-  forall f tf (Hsim: fundef_sig_sim f tf),
+  forall f tf (Hsim: fundef_sig_lsim f tf),
     fundef_sig_src f = fundef_sig_tgt tf.
 Proof.
   intros. inv Hsim. auto.
@@ -612,4 +612,4 @@ Qed.
 
 End INITIALIZE.
 
-End PROGRAM_SIM.
+End PROGRAM_LSIM.
