backend/RTLLSim.v
@@ -1,0 +1,205 @@
+Require Import RelationClasses.
+Require Import Coqlib.
+Require Import paco.
+Require Import WFType.
+Require Import Maps.
+Require Import AST.
+Require Import Integers.
+Require Import Values.
+Require Import Events.
+Require Import Memory.
+Require Import Globalenvs.
+Require Import Smallstep.
+Require Import Op.
+Require Import Registers.
+Require Import RTL.
+Require Import LinkerSpecification.
+Require Import ProgramLSim.
+Require Import ValueAnalysis_linker.
+
+Set Implicit Arguments.
+
+Definition state_mem (st:state): mem :=
+  match st with
+    | State _ _ _ _ _ m => m
+    | Callstate _ _ _ m => m
+    | Returnstate _ _ m => m
+  end.
+
+(* memory relation *)
+
+Record mrelT_opsT (t:Type): Type := mkmrelT_opsT {
+  sem :> t -> forall (i:WF.t) (s1 s2:state), Prop;
+  sem_value :> t -> forall (v1 v2:val), Prop;
+  le: t -> t -> Prop;
+  le_public: t -> t -> Prop
+}.
+
+Record mrelT_propsT (t:Type) (ops:mrelT_opsT t): Prop := mkmrelT_propsT {
+  le_preorder: PreOrder ops.(le);
+  le_public_preorder: PreOrder ops.(le_public);
+  le_public_le:
+    forall mrel1 mrel2 (Hle_public: ops.(le_public) mrel1 mrel2),
+      ops.(le) mrel1 mrel2;
+  sem_value_int:
+    forall mrel i v (H: ops.(sem_value) mrel (Vint i) v),
+      v = Vint i
+
+}.
+
+(* memory relation - equals *)
+
+Definition mrelT_ops_equals: mrelT_opsT unit :=
+  mkmrelT_opsT
+    (fun _ _ s1 s2 => state_mem s1 = state_mem s2)
+    (fun _ v1 v2 => Val.lessdef v1 v2)
+    (fun _ _ => True)
+    (fun _ _ => True).
+
+Program Definition mrelT_props_equals: mrelT_propsT mrelT_ops_equals := mkmrelT_propsT _ _ _ _ _.
+Next Obligation. repeat constructor. Qed.
+Next Obligation. repeat constructor. Qed.
+Next Obligation. inv H. auto. Qed.
+
+(* memory relation - extends *)
+
+Definition mrelT_ops_extends: mrelT_opsT unit :=
+  mkmrelT_opsT
+    (fun _ _ s1 s2 => Mem.extends (state_mem s1) (state_mem s2))
+    (fun _ v1 v2 => Val.lessdef v1 v2)
+    (fun _ _ => True)
+    (fun _ _ => True).
+
+Program Definition mrelT_props_extends: mrelT_propsT mrelT_ops_extends := mkmrelT_propsT _ _ _ _ _.
+Next Obligation. repeat constructor. Qed.
+Next Obligation. repeat constructor. Qed.
+Next Obligation. inv H. auto. Qed.
+
+Lemma mrelT_ops_extends_lessdef_list mrel v1 v2:
+  Val.lessdef_list v1 v2 <-> list_forall2 (mrelT_ops_extends.(sem_value) mrel) v1 v2.
+Proof.
+  revert v2.
+  induction v1; intros; constructor; intro H; inv H; constructor; auto.
+  - apply IHv1. auto.
+  - apply IHv1. auto.
+Qed.
+
+Section LSIM.
+
+Variable (mrelT:Type).
+Variable (mrelT_ops:mrelT_opsT mrelT).
+
+Variable (fprog_src fprog_tgt:program).
+
+Let ge_src := Genv.globalenv fprog_src.
+Let ge_tgt := Genv.globalenv fprog_tgt.
+
+Section STATE_LSIM.
+
+Variable (cs_entry_src cs_entry_tgt:list stackframe).
+Variable (mrel_entry:mrelT).
+
+Inductive _state_lsim_or_csim
+          (state_lsim: mrelT -> WF.t -> state -> state -> Prop)
+          (mrel:mrelT) (i:WF.t) (st_src st_tgt:state): Prop :=
+| _state_lsim_or_csim_lsim
+    (Hlsim: state_lsim mrel i st_src st_tgt)
+| _state_lsim_or_csim_csim
+    stack_src fundef_src args_src mem_src
+    (Hst_src: st_src = Callstate stack_src fundef_src args_src mem_src)
+    stack_tgt fundef_tgt args_tgt mem_tgt
+    (Hst_tgt: st_tgt = Callstate stack_tgt fundef_tgt args_tgt mem_tgt)
+    (Hfundef: fundef_weak_lsim
+                (@common_fundef_dec function) fn_sig
+                (@common_fundef_dec function) fn_sig
+                ge_src ge_tgt fundef_src fundef_tgt)
+    (Hargs: list_forall2 (mrelT_ops.(sem_value) mrel) args_src args_tgt)
+    (Hmrel: mrelT_ops.(sem) mrel i st_src st_tgt)
+    (Hreturn:
+       forall mrel2 i2 st2_src st2_tgt mem2_src mem2_tgt vres_src vres_tgt
+              (Hvres: mrelT_ops.(sem_value) mrel2 vres_src vres_tgt)
+              (Hst2_src: st2_src = Returnstate stack_src vres_src mem2_src)
+              (Hst2_tgt: st2_tgt = Returnstate stack_tgt vres_tgt mem2_tgt)
+              (Hsound_src: sound_state_ext fprog_src st2_src)
+              (Hsound_tgt: sound_state_ext fprog_tgt st2_tgt)
+              (Hmrel2_le: mrelT_ops.(le_public) mrel mrel2)
+              (Hst2_mem: mrelT_ops.(sem) mrel2 i2 st2_src st2_tgt),
+         state_lsim mrel2 i2 st2_src st2_tgt)
+.
+
+Inductive _state_lsim
+          (state_lsim: mrelT -> WF.t -> state -> state -> Prop)
+          (mrel:mrelT) (i:WF.t) (st_src st_tgt:state): Prop :=
+| _state_lsim_term
+    rval
+    (Hst_src: final_state st_src rval)
+    (Hst_tgt: final_state st_tgt rval)
+
+| _state_lsim_return
+    (Hsound_src: sound_state_ext fprog_src st_src)
+    (Hsound_tgt: sound_state_ext fprog_tgt st_tgt)
+    val_src mem_src (Hst_src: st_src = Returnstate cs_entry_src val_src mem_src)
+    val_tgt mem_tgt (Hst_tgt: st_tgt = Returnstate cs_entry_tgt val_tgt mem_tgt)
+    (Hval: mrelT_ops.(sem_value) mrel val_src val_tgt)
+    (Hmem: mrelT_ops.(sem) mrel i st_src st_tgt)
+    (Hmrel_le_public: mrelT_ops.(le_public) mrel_entry mrel)
+
+| _state_lsim_step
+    (Hnfinal: forall r, ~ final_state st_src r)
+    (Hsound_src: sound_state_ext fprog_src st_src)
+    (Hsound_tgt: sound_state_ext fprog_tgt st_tgt)
+    (Hpreserve:
+       forall evt st2_src (Hst2_src: step ge_src st_src evt st2_src),
+         exists i2 st2_tgt (mrel2:mrelT),
+           (plus step ge_tgt st_tgt evt st2_tgt \/
+            star step ge_tgt st_tgt evt st2_tgt /\ WF.rel i2 i) /\
+           mrelT_ops.(le) mrel mrel2 /\
+           mrelT_ops.(sem) mrel2 i2 st2_src st2_tgt /\
+           _state_lsim_or_csim state_lsim mrel2 i2 st2_src st2_tgt)
+.
+Hint Constructors _state_lsim.
+
+Lemma state_lsim_mon: monotone4 _state_lsim.
+Proof.
+  repeat intro; destruct IN; eauto.
+  - eapply _state_lsim_step; eauto.
+    intros. exploit Hpreserve; eauto. intros [i2 [st2_tgt [mrel2 [Hstep [Hle [Hmrel Hsim]]]]]].
+    eexists. eexists. eexists. repeat (split; eauto).
+    inv Hsim.
+    + apply _state_lsim_or_csim_lsim. eauto.
+    + eapply _state_lsim_or_csim_csim; eauto.
+Qed.
+
+Definition state_lsim: _ -> _ -> _ -> _ -> Prop :=
+  paco4 _state_lsim bot4.
+
+End STATE_LSIM.
+
+Inductive function_lsim (func_src func_tgt:function): Prop :=
+| function_lsim_intro
+    (Hlsim:
+       forall
+         mrel_init
+         mrel_entry mem_entry_src mem_entry_tgt
+         cs_entry_src cs_entry_tgt
+         args_src args_tgt
+         st_src st_tgt
+         i
+         (Hmrel_init: True) (* TODO *)
+         (Hmrel_entry_le: mrelT_ops.(le) mrel_init mrel_entry)
+         (Hmrel_entry: mrelT_ops.(sem) mrel_entry i st_src st_tgt)
+         (Hargs: list_forall2 (mrelT_ops.(sem_value) mrel_entry) args_src args_tgt)
+         (Hst_src: st_src = (Callstate cs_entry_src (Internal func_src) args_src mem_entry_src))
+         (Hst_tgt: st_tgt = (Callstate cs_entry_tgt (Internal func_tgt) args_tgt mem_entry_tgt))
+         (Hsound_src: sound_state_ext fprog_src st_src)
+         (Hsound_tgt: sound_state_ext fprog_tgt st_tgt),
+         state_lsim
+           cs_entry_src cs_entry_tgt mrel_entry
+           mrel_entry i
+           (Callstate cs_entry_src (Internal func_src) args_src mem_entry_src)
+           (Callstate cs_entry_tgt (Internal func_tgt) args_tgt mem_entry_tgt))
+.
+
+End LSIM.
+Hint Constructors _state_lsim.
+Hint Resolve state_lsim_mon: paco.
